# Variation notation
$$ 
1. V_1(a, b) = a^b\\
2. V_n(a, b) = V_{n-1}(\underbrace{a, a, a ... a}_b)\\
3. V_n(P, 0, Q) = V_n(P, Q)\\
4. V_n(P, 1) = V_n(P)\\
\text{if not do rules 1 - 4} \\
5. V_n(a_1, a_2, a_3...a_k) = \\
V_n
(
    V_n(a_1, a_2 - 1, a_3, a_4, ... a_k), \\
    V_n(a_1, a_2, a_3 - 1, a_4, ... a_k), \\
    V_n(a_1, a_2, a_3, a_4 - 1, ... a_k)...
    V_n(a_1, a_2, a_3, a_4,...a_k - 1)
)\\
P \ and \ Q  - vectors\\
V_1(3, 2) = 3^2 = 9 \\
V_1(2, 2, 2) =...
$$
Calculation.
Variations array {2, 2, 2} :
$$
\begin{array}{l}
V_1(2, 2, 2) : \\
V_1(2, 2 - 1, 2) = V_1(2, 1, 2) \\
V_1(2, 2, 2 - 1) = (2, 2, 1) = (2, 2) = 2^2 = 4 \\
V_1(2, 1, 2) : \\
V_1(2, 0, 2) = (2, 2) = 4 \\
V_1(2, 1, 1) = 2 \\
V_1(2, 1, 2) = V_1(4, 2) = 16 \\
V_1(2, 2, 2) = V_2(2, 3) = V_1(V_1(2, 1, 2) = 16, V_1(2, 2, 1) = 4) \\
16^4 = 65536 \\
V_2(2, 3) = V_1(2, 2, 2) = 65536 \\
V_2(2, 4) = V_1(2, 2, 2, 2) = \\
V_1(V_1(2, 1, 2, 2), V_1(2, 2, 1, 2), V_1(2, 2, 2, 1)
= V_1(2, 2, 2)) = \\
V_1(V_1(2, 1, 2, 2), V_1(2, 2, 1, 2), 65536) = \\
V_1(2, 1, 2, 2) = V_1(65536, V_1(16, 16, 2), 16) \\
V_1(2, 1, 1, 2) = V_1(16, 16, 2) \\
V_1(2, 2, 1, 2) = V_1(V_1(2, 1, 1, 2), V_1(2, 2,  2) = 
65536, V(2, 2) = 4) = \\
V_1(V_1(16, 16, 2), 65536, 4) \\
V_2(3, 2, 3) = 27
\end{array}
$$
## Vector variation notation
$$
 \begin{array}{l}
V_{[2, 2]}(2, 2) = V_{[4, 1]}^2(2, 2) = V_{[4, 1]}(V_{[4, 1]}(2, 2), 2) = V_{[4, 1]}(V_{[4]}(2, 2), 2)\\ = V_{[4]}(V_{[4]}(2, 2), 2) = 
V_4(V_4(2, 2), 2) = V_4(4, 2) = 
V_3(4, 4) =\\ V_2(4, 4, 4, 4) = Vi([[2, 2], [2, 2]])\\
V_{[a]}(P) = V_a(P)\\
V_{[a, b]}(P) = V\\
V_{[P, 1]}(Q) = V_P(Q)\\
V_{[P, 0, Q]}(N) = V_{[P, Q]}(N)\\
V_{[a_1, a_2, a_3, a_4..., a_k]_n}(b_1, b_2, b_3, b_4..., b_m) = \\
{[{V^k}_n(a_1, a_2 - 1, a_3,a_4,... a_k), V_n(a_1, a_2, a_3 - 1, a_4,... a_k),
 V_n(a_1, a_2, a_3,a_4-1), ..., V_n(a_1...a_{k-1}-1, a_k), a_k-1]}\\
 (b_1, b_2, b_3, b_4,... b_m)\\
 V_P^n(a_1, a_2, a_3...a_m)
 \underbrace{V_P(a_1, a_2..., V_P(a_1, a_2...,V_P
 (...)))...}_n\\
\end{array}
$$